examples/cms/verif_CMS_clear.v
@@ -230,7 +230,7 @@ Proof.
     step_into.
     { hoare_func_table; elim_trivial_cases.
       { clear -H5; lia. }
-      table_action NoAction_body.
+      table_action (@NoAction_body Info).
       { entailer. }
       { apply arg_ret_implies_refl. }
     }
@@ -263,7 +263,7 @@ Proof.
     step_into.
     { hoare_func_table; elim_trivial_cases.
       { clear -H5; lia. }
-      table_action NoAction_body.
+      table_action (@NoAction_body Info).
       { entailer. }
       { apply arg_ret_implies_refl. }
     }
@@ -296,7 +296,7 @@ Proof.
     step_into.
     { hoare_func_table; elim_trivial_cases.
       { clear -H5; lia. }
-      table_action NoAction_body.
+      table_action (@NoAction_body Info).
       { entailer. }
       { apply arg_ret_implies_refl. }
     }
