examples/sbf/verif_Filter_insert.v
@@ -236,7 +236,7 @@ Proof.
     simpl Z.eqb. cbn match.
     step_into.
     { hoare_func_table_nondet; elim_trivial_cases.
-      table_action NoAction_body.
+      table_action (@NoAction_body Info).
       { entailer. }
       { apply arg_ret_implies_refl. }
     }
@@ -266,7 +266,7 @@ Proof.
     simpl Z.eqb. cbn match.
     step_into.
     { hoare_func_table_nondet; elim_trivial_cases.
-      table_action NoAction_body.
+      table_action (@NoAction_body Info).
       { entailer. }
       { apply arg_ret_implies_refl. }
     }
@@ -296,7 +296,7 @@ Proof.
     simpl Z.eqb. cbn match.
     step_into.
     { hoare_func_table_nondet; elim_trivial_cases.
-      table_action NoAction_body.
+      table_action (@NoAction_body Info).
       { entailer. }
       { apply arg_ret_implies_refl. }
     }
@@ -326,7 +326,7 @@ Proof.
     simpl Z.eqb. cbn match.
     step_into.
     { hoare_func_table_nondet; elim_trivial_cases.
-      table_action NoAction_body.
+      table_action (@NoAction_body Info).
       { entailer. }
       { apply arg_ret_implies_refl. }
     }
